completed liveness total mappings

core/TotalMapLivenessSimulations.v
@@ -12,6 +12,7 @@ Require Import StructTact.Util.
 
 Require Import TotalMapSimulations.
 Require Import infseq.
+Require Import FunctionalExtensionality.
 
 Local Arguments update {_} {_} {_} _ _ _ _ : simpl never.
 
@@ -58,6 +59,14 @@ Class LabeledMultiParamsTotalMapCongruency
       tot_mapped_lb_input_handlers_label me inp st = lb ;
     tot_lb_label_silent_fst_snd : tot_map_label label_silent = label_silent
   }.
+
+Lemma prod_fst_snd_eq : 
+  forall A B (ab : A * B),
+    ab = (fst ab, snd ab).
+Proof.
+move => A B ab.
+by destruct ab.
+Qed.
 
 Section TotalMapLivenessSimulations.
 
@@ -118,47 +127,159 @@ invcs H_step => //=.
   exact: LSF_stutter.
 Qed.
 
-Definition tot_map_event_state e :=
+Theorem lb_step_o_f_tot_mapped_simulation_1 :
+  forall net net' failed failed' lb tr,
+    @lb_step_o_f _ labeled_multi_fst (failed, net) lb (failed', net') tr ->
+    @lb_step_o_f _ labeled_multi_snd (map tot_map_name failed, tot_map_onet net) (tot_map_label lb) (map tot_map_name failed', tot_map_onet net') (map tot_map_trace_occ tr).
+Proof.
+move => net net' failed failed' lb tr H_step.
+invcs H_step => //=.
+- apply (@LSOF_deliver _ _ _ _ _ (@tot_map_msg _ _ _ _ msg_map m) (map (@tot_map_msg _ _ _ _ msg_map) ms) _ (tot_map_data d) (@tot_map_name_msgs _ _ _ _ _ msg_map l) (@tot_map_name _ _ _ _ name_map from)).
+  * rewrite /tot_map_onet /=.
+    rewrite 2!tot_map_name_inv_inverse.
+    by find_rewrite.
+  * exact: not_in_failed_not_in.
+  * rewrite /tot_map_onet /= tot_map_name_inv_inverse.
+    have H_q := @tot_net_handlers_eq _ _ _ _ _ _ _ multi_map_congr to from m (onwState net to).
+    rewrite /tot_mapped_net_handlers /net_handlers /= /unlabeled_net_handlers in H_q.
+    repeat break_let.
+    repeat tuple_inversion.
+    have H_q' := @tot_lb_net_handlers_eq _ _ _ _ _ _ _ _ multi_map_lb_congr _ _ _ _ _ _ _ _ Heqp1.
+    rewrite /tot_mapped_lb_net_handlers_label in H_q'.
+    repeat break_let.
+    by repeat tuple_inversion.
+  * rewrite /tot_map_onet /=.         
+    rewrite (@collate_tot_map_update2_eq _ _ _ _ _ _ name_map_bijective).
+    set f1 := fun _ => tot_map_data _.
+    set f2 := update' _ _ _.
+    have H_eq_f: f1 = f2.
+      rewrite /f1 /f2.
+      apply functional_extensionality => n.
+      rewrite /update'.
+      break_if; break_if => //; first by rewrite -e tot_map_name_inverse_inv in n0.
+      by rewrite e tot_map_name_inv_inverse in n0.
+    by rewrite H_eq_f.
+- rewrite /tot_map_onet /=.
+  apply (@LSOF_input _ _ _ _ _ _ _ _ (tot_map_data d) (@tot_map_name_msgs _ _ _ _ _ msg_map l)).
+  * exact: not_in_failed_not_in.
+  * rewrite /tot_map_onet /= tot_map_name_inv_inverse.
+    have H_q := @tot_input_handlers_eq _ _ _ _ _ _ _ multi_map_congr h inp (onwState net h).
+    rewrite /tot_mapped_input_handlers /= /unlabeled_input_handlers in H_q.
+    repeat break_let.
+    repeat tuple_inversion.
+    have H_q' := @tot_lb_input_handlers_eq _ _ _ _ _ _ _ _ multi_map_lb_congr _ _ _ _ _ _ _ Heqp1.
+    rewrite /tot_mapped_lb_input_handlers_label in H_q'.
+    repeat break_let.
+    by repeat tuple_inversion.
+  * rewrite /tot_map_onet /=.
+    rewrite (@collate_tot_map_eq _ _ _ _ _ _ name_map_bijective).
+    set f1 := fun _ => tot_map_data _.
+    set f2 := update' _ _ _.
+    have H_eq_f: f1 = f2.
+      rewrite /f1 /f2.
+      apply functional_extensionality => n.
+      rewrite /update'.
+      break_if; break_if => //; first by rewrite -e tot_map_name_inverse_inv in n0.
+      by rewrite e tot_map_name_inv_inverse in n0.
+    by rewrite H_eq_f.
+- rewrite tot_lb_label_silent_fst_snd.
+  exact: LSOF_stutter.
+Qed.
+
+Theorem lb_step_o_d_f_tot_mapped_simulation_1 :
+  forall net net' failed failed' lb tr,
+    @lb_step_o_d_f _ labeled_multi_fst (failed, net) lb (failed', net') tr ->
+    @lb_step_o_d_f _ labeled_multi_snd (map tot_map_name failed, tot_map_odnet net) (tot_map_label lb) (map tot_map_name failed', tot_map_odnet net') (map tot_map_trace_occ tr).
+Proof.
+move => net net' failed failed' lb tr H_step.
+invcs H_step => //=.
+- rewrite /tot_map_odnet /=.
+  apply (@LSODF_deliver _ _ _ _ _ (@tot_map_msg _ _ _ _ msg_map m) (map (@tot_map_msg _ _ _ _ msg_map) ms) _ (tot_map_data d) (tot_map_data d') (@tot_map_name_msgs _ _ _ _ _ msg_map l) (@tot_map_name _ _ _ _ name_map from)) => //=.
+  * exact: not_in_failed_not_in.
+  * exact: in_failed_in. 
+  * rewrite tot_map_name_inv_inverse.
+    by find_rewrite.
+  * rewrite 2!tot_map_name_inv_inverse.
+    by find_rewrite.
+  * have H_q := @tot_net_handlers_eq _ _ _ _ _ _ _ multi_map_congr to from m d.
+    rewrite /tot_mapped_net_handlers /net_handlers /= /unlabeled_net_handlers in H_q.
+    repeat break_let.
+    repeat tuple_inversion.
+    have H_q' := @tot_lb_net_handlers_eq _ _ _ _ _ _ _ _ multi_map_lb_congr _ _ _ _ _ _ _ _ Heqp1.
+    rewrite /tot_mapped_lb_net_handlers_label in H_q'.
+    repeat break_let.
+    by repeat tuple_inversion.
+  * rewrite (@collate_tot_map_update2_eq _ _ _ _ _ _ name_map_bijective).
+    set f1 := fun _ => match _ with _ => _ end.
+    set f2 := update_opt _ _ _.
+    have H_eq_f: f1 = f2.
+      rewrite /f1 /f2 /update_opt.
+      apply functional_extensionality => dst.
+      repeat break_if => //=; first by rewrite -e tot_map_name_inverse_inv in n.
+      by rewrite e tot_map_name_inv_inverse in n.
+    by rewrite H_eq_f.
+- rewrite /tot_map_odnet /=.
+  apply (@LSODF_input _ _ _ _ _ _ _ _ (tot_map_data d) (tot_map_data d') (@tot_map_name_msgs _ _ _ _ _ msg_map l)) => //=.
+  * exact: not_in_failed_not_in.
+  * exact: in_failed_in. 
+  * rewrite tot_map_name_inv_inverse.
+    by find_rewrite.
+  * have H_q := @tot_input_handlers_eq _ _ _ _ _ _ _ multi_map_congr h inp d.
+    rewrite /tot_mapped_input_handlers /= /unlabeled_input_handlers in H_q.
+    repeat break_let.
+    repeat tuple_inversion.
+    have H_q' := @tot_lb_input_handlers_eq _ _ _ _ _ _ _ _ multi_map_lb_congr _ _ _ _ _ _ _ Heqp1.
+    rewrite /tot_mapped_lb_input_handlers_label in H_q'.
+    repeat break_let.
+    by repeat tuple_inversion.
+  * rewrite (@collate_tot_map_eq _ _ _ _ _ _ name_map_bijective).
+    set f1 := fun _ => match _ with _ => _ end.
+    set f2 := update_opt _ _ _.
+    have H_eq_f: f1 = f2.
+      rewrite /f1 /f2 /update_opt.
+      apply functional_extensionality => n.
+      repeat break_match; try by congruence.
+      * by rewrite e tot_map_name_inv_inverse in n0.
+      * by rewrite -e tot_map_name_inverse_inv in n0.
+      * by rewrite e tot_map_name_inv_inverse in n0.
+    by rewrite H_eq_f.
+- rewrite tot_lb_label_silent_fst_snd.
+  exact: LSODF_stutter.
+Qed.
+
+Definition tot_map_net_event_state e :=
 {| evt_r_a := (map tot_map_name (fst e.(evt_r_a)), tot_map_net (snd e.(evt_r_a))) ;
    evt_r_l := tot_map_label e.(evt_r_l) |}.
 
-Lemma tot_map_event_state_Map_unfold : forall s,
- Cons (tot_map_event_state (hd s)) (Map tot_map_event_state (tl s)) = Map tot_map_event_state s.
+Lemma tot_map_net_event_state_Map_unfold : forall s,
+ Cons (tot_map_net_event_state (hd s)) (Map tot_map_net_event_state (tl s)) = Map tot_map_net_event_state s.
 Proof.
 by move => s; rewrite -Map_Cons /= -{3}(recons s).
 Qed.
-
-Lemma prod_fst_snd_eq : 
-  forall A B (ab : A * B),
-    ab = (fst ab, snd ab).
-Proof.
-move => A B ab.
-by destruct ab.
-Qed.
   
-Lemma lb_step_execution_lb_step_f_tot_map_infseq : forall s,
+Lemma lb_step_state_execution_lb_step_f_tot_map_net_infseq : forall s,
   lb_step_state_execution lb_step_f s ->
-  lb_step_state_execution lb_step_f (Map tot_map_event_state s).
+  lb_step_state_execution lb_step_f (Map tot_map_net_event_state s).
 Proof.
 cofix c.
 move => s H_exec.
-rewrite -tot_map_event_state_Map_unfold {1}/tot_map_event_state /=.
+rewrite -tot_map_net_event_state_Map_unfold {1}/tot_map_net_event_state /=.
 inversion H_exec; subst => /=.
-rewrite -tot_map_event_state_Map_unfold /= /tot_map_event_state /=.
+rewrite -tot_map_net_event_state_Map_unfold /= /tot_map_net_event_state /=.
 apply: (@Cons_lb_step_exec _ _ _ _ _ _ _ _ (map tot_map_trace_occ tr)) => /=.
 - apply: lb_step_f_tot_mapped_simulation_1.
   by rewrite -2!prod_fst_snd_eq.
 - set e0 := {| evt_r_a := _ ; evt_r_l := _  |}.
-  have ->: e0 = tot_map_event_state e' by [].
+  have ->: e0 = tot_map_net_event_state e' by [].
   pose s' := Cons e' s0.
-  rewrite (tot_map_event_state_Map_unfold s').
+  rewrite (tot_map_net_event_state_Map_unfold s').
   exact: c.
 Qed.
 
-Lemma tot_map_label_event_state_inf_often_occurred :
+Lemma tot_map_net_label_event_state_inf_often_occurred :
   forall l s,
     inf_often (now (occurred l)) s ->
-    inf_often (now (occurred (tot_map_label l))) (Map tot_map_event_state s).
+    inf_often (now (occurred (tot_map_label l))) (Map tot_map_net_event_state s).
 Proof.
 move => l.
 apply: always_Map.
@@ -172,9 +293,9 @@ Qed.
 Hypothesis tot_map_label_injective : 
   forall l l', tot_map_label l = tot_map_label l' -> l = l'.
 
-Lemma tot_map_label_event_state_inf_often_occurred_conv :
+Lemma tot_map_net_label_event_state_inf_often_occurred_conv :
   forall l s,
-    inf_often (now (occurred (tot_map_label l))) (Map tot_map_event_state s) ->
+    inf_often (now (occurred (tot_map_label l))) (Map tot_map_net_event_state s) ->
     inf_often (now (occurred l)) s.
 Proof.
 move => l.
@@ -196,26 +317,26 @@ apply: eventually_Map_conv => //.
   exact: tot_map_label_injective.
 Qed.
 
-Definition tot_map_event_state_trace e :=
+Definition tot_map_net_event_state_trace e :=
 {| evt_tr_r_a := (map tot_map_name (fst e.(evt_tr_r_a)), tot_map_net (snd e.(evt_tr_r_a))) ;
    evt_tr_r_l := tot_map_label e.(evt_tr_r_l) ;
    evt_tr_r_trace := map tot_map_trace_occ e.(evt_tr_r_trace) |}.
 
-Lemma tot_map_event_state_trace_Map_unfold : forall s,
- Cons (tot_map_event_state_trace (hd s)) (Map tot_map_event_state_trace (tl s)) = Map tot_map_event_state_trace s.
+Lemma tot_map_net_event_state_trace_Map_unfold : forall s,
+ Cons (tot_map_net_event_state_trace (hd s)) (Map tot_map_net_event_state_trace (tl s)) = Map tot_map_net_event_state_trace s.
 Proof.
 by move => s; rewrite -Map_Cons /= -{3}(recons s).
 Qed.
 
-Lemma lb_step_trace_execution_lb_step_f_tot_map_infseq : forall s,
+Lemma lb_step_trace_execution_lb_step_f_tot_map_net_infseq : forall s,
   lb_step_state_trace_execution lb_step_f s ->
-  lb_step_state_trace_execution lb_step_f (Map tot_map_event_state_trace s).
+  lb_step_state_trace_execution lb_step_f (Map tot_map_net_event_state_trace s).
 Proof.
 cofix c.
 move => s H_exec.
-rewrite -tot_map_event_state_trace_Map_unfold {1}/tot_map_event_state_trace /=.
+rewrite -tot_map_net_event_state_trace_Map_unfold {1}/tot_map_net_event_state_trace /=.
 inversion H_exec; subst => /=.
-rewrite -tot_map_event_state_trace_Map_unfold /= /tot_map_event_state_trace /=.
+rewrite -tot_map_net_event_state_trace_Map_unfold /= /tot_map_net_event_state_trace /=.
 apply: (@Cons_lb_step_trace_exec _ _ _ _ _ _ _ _ (map tot_map_trace_occ tr)) => /=.
 - apply: lb_step_f_tot_mapped_simulation_1.
   by rewrite -2!prod_fst_snd_eq.
@@ -223,16 +344,16 @@ apply: (@Cons_lb_step_trace_exec _ _ _ _ _ _ _ _ (map tot_map_trace_occ tr)) => 
   find_rewrite.
   by rewrite map_app.
 - set e0 := {| evt_tr_r_a := _ ; evt_tr_r_l := _ ; evt_tr_r_trace := _ |}.
-  have ->: e0 = tot_map_event_state_trace e' by [].
+  have ->: e0 = tot_map_net_event_state_trace e' by [].
   pose s' := Cons e' s0.
-  rewrite (tot_map_event_state_trace_Map_unfold s').
+  rewrite (tot_map_net_event_state_trace_Map_unfold s').
   exact: c.
 Qed.
 
-Lemma tot_map_label_event_state_trace_inf_often_occurred :
+Lemma tot_map_net_label_event_state_trace_inf_often_occurred :
   forall l s,
     inf_often (now (occurred l)) s ->
-    inf_often (now (occurred (tot_map_label l))) (Map tot_map_event_state_trace s).
+    inf_often (now (occurred (tot_map_label l))) (Map tot_map_net_event_state_trace s).
 Proof.
 move => l.
 apply: always_Map.
@@ -243,9 +364,9 @@ move => H_eq.
 by rewrite H_eq.
 Qed.
 
-Lemma tot_map_label_event_state_trace_inf_often_occurred_conv :
+Lemma tot_map_net_label_event_state_trace_inf_often_occurred_conv :
   forall l s,
-    inf_often (now (occurred (tot_map_label l))) (Map tot_map_event_state_trace s) ->
+    inf_often (now (occurred (tot_map_label l))) (Map tot_map_net_event_state_trace s) ->
     inf_often (now (occurred l)) s.
 Proof.
 move => l.
@@ -271,34 +392,382 @@ Context {fail_fst : FailureParams (@unlabeled_multi_params _ labeled_multi_fst)}
 Context {fail_snd : FailureParams (@unlabeled_multi_params _ labeled_multi_snd)}.
 Context {fail_map_congr : FailureParamsTotalMapCongruency fail_fst fail_snd base_map}.
 
-Lemma tot_map_hd_step_f_star_ex_always : 
+Lemma tot_map_net_hd_step_f_star_ex_always : 
   forall s, event_step_star_ex step_f step_f_init (hd s) ->
        lb_step_state_execution lb_step_f s ->
-       always (now (event_step_star_ex step_f step_f_init)) (Map tot_map_event_state s).
+       always (now (event_step_star_ex step_f step_f_init)) (Map tot_map_net_event_state s).
 Proof.
 case => e s H_star H_exec.
 apply: step_f_star_ex_lb_step_state_execution.
-  rewrite /= /tot_map_event_state /= /event_step_star_ex /=.
-  rewrite /= /tot_map_event_state /= /event_step_star_ex /= in H_star.
+  rewrite /= /tot_map_net_event_state /= /event_step_star_ex /=.
+  rewrite /= /tot_map_net_event_state /= /event_step_star_ex /= in H_star.
   break_exists.
   exists (map (@tot_map_trace_occ _ _ _ _ _ name_map) x).
   apply: step_f_tot_mapped_simulation_star_1 => //.
   by rewrite -prod_fst_snd_eq.  
-exact: lb_step_execution_lb_step_f_tot_map_infseq.
+exact: lb_step_state_execution_lb_step_f_tot_map_net_infseq.
 Qed.
 
-Lemma tot_map_hd_step_f_star_always : 
+Lemma tot_map_net_hd_step_f_star_always : 
   forall s, event_step_star step_f step_f_init (hd s) ->
        lb_step_state_trace_execution lb_step_f s ->
-       always (now (event_step_star step_f step_f_init)) (Map tot_map_event_state_trace s).
+       always (now (event_step_star step_f step_f_init)) (Map tot_map_net_event_state_trace s).
 Proof.
 case => e s H_star H_exec.
 apply: step_f_star_lb_step_state_trace_execution.
   rewrite /=.
-  rewrite /tot_map_event_state_trace /= /event_step_star /=.
+  rewrite /tot_map_net_event_state_trace /= /event_step_star /=.
   apply: step_f_tot_mapped_simulation_star_1.
   by rewrite -prod_fst_snd_eq.
-exact: lb_step_trace_execution_lb_step_f_tot_map_infseq.
+exact: lb_step_trace_execution_lb_step_f_tot_map_net_infseq.
+Qed.
+
+Definition tot_map_onet_event_state e :=
+{| evt_r_a := (map tot_map_name (fst e.(evt_r_a)), tot_map_onet (snd e.(evt_r_a))) ;
+   evt_r_l := tot_map_label e.(evt_r_l) |}.
+
+Lemma tot_map_onet_event_state_Map_unfold : forall s,
+ Cons (tot_map_onet_event_state (hd s)) (Map tot_map_onet_event_state (tl s)) = Map tot_map_onet_event_state s.
+Proof.
+by move => s; rewrite -Map_Cons /= -{3}(recons s).
+Qed.
+
+Lemma lb_step_state_execution_lb_step_o_f_tot_map_onet_infseq : forall s,
+  lb_step_state_execution lb_step_o_f s ->
+  lb_step_state_execution lb_step_o_f (Map tot_map_onet_event_state s).
+Proof.
+cofix c.
+move => s H_exec.
+rewrite -tot_map_onet_event_state_Map_unfold {1}/tot_map_onet_event_state /=.
+inversion H_exec; subst => /=.
+rewrite -tot_map_onet_event_state_Map_unfold /= /tot_map_onet_event_state /=.
+apply: (@Cons_lb_step_exec _ _ _ _ _ _ _ _ (map tot_map_trace_occ tr)) => /=.
+- apply: lb_step_o_f_tot_mapped_simulation_1.
+  by rewrite -2!prod_fst_snd_eq.
+- set e0 := {| evt_r_a := _ ; evt_r_l := _  |}.
+  have ->: e0 = tot_map_onet_event_state e' by [].
+  pose s' := Cons e' s0.
+  rewrite (tot_map_onet_event_state_Map_unfold s').
+  exact: c.
+Qed.
+
+Lemma tot_map_onet_label_event_state_inf_often_occurred :
+  forall l s,
+    inf_often (now (occurred l)) s ->
+    inf_often (now (occurred (tot_map_label l))) (Map tot_map_onet_event_state s).
+Proof.
+move => l.
+apply: always_Map.
+apply: eventually_Map.
+case => e s.
+rewrite /= /occurred /evt_l /=.
+move => H_eq.
+by rewrite H_eq.
+Qed.
+
+Lemma tot_map_onet_label_event_state_inf_often_occurred_conv :
+  forall l s,
+    inf_often (now (occurred (tot_map_label l))) (Map tot_map_onet_event_state s) ->
+    inf_often (now (occurred l)) s.
+Proof.
+move => l.
+apply: always_Map_conv.
+apply: eventually_Map_conv => //.
+- rewrite /extensional /=.
+  case => e s1.
+  case => e' s2.
+  move => H_eq.
+  by inversion H_eq; subst_max.
+- rewrite /extensional /=.
+  case => e s1.
+  case => e' s2.
+  move => H_eq.
+  by inversion H_eq; subst_max.
+- case => e s.
+  rewrite /= /occurred /=.
+  move => H_eq.
+  exact: tot_map_label_injective.
+Qed.
+
+Definition tot_map_onet_event_state_trace e :=
+{| evt_tr_r_a := (map tot_map_name (fst e.(evt_tr_r_a)), tot_map_onet (snd e.(evt_tr_r_a))) ;
+   evt_tr_r_l := tot_map_label e.(evt_tr_r_l) ;
+   evt_tr_r_trace := map tot_map_trace_occ e.(evt_tr_r_trace) |}.
+
+Lemma tot_map_onet_event_state_trace_Map_unfold : forall s,
+ Cons (tot_map_onet_event_state_trace (hd s)) (Map tot_map_onet_event_state_trace (tl s)) = Map tot_map_onet_event_state_trace s.
+Proof.
+by move => s; rewrite -Map_Cons /= -{3}(recons s).
+Qed.
+
+Lemma lb_step_state_trace_execution_lb_step_o_f_tot_map_onet_infseq : forall s,
+  lb_step_state_trace_execution lb_step_o_f s ->
+  lb_step_state_trace_execution lb_step_o_f (Map tot_map_onet_event_state_trace s).
+Proof.
+cofix c.
+move => s H_exec.
+rewrite -tot_map_onet_event_state_trace_Map_unfold {1}/tot_map_onet_event_state_trace /=.
+inversion H_exec; subst => /=.
+rewrite -tot_map_onet_event_state_trace_Map_unfold /= /tot_map_onet_event_state_trace /=.
+apply: (@Cons_lb_step_trace_exec _ _ _ _ _ _ _ _ (map tot_map_trace_occ tr)) => /=.
+- apply: lb_step_o_f_tot_mapped_simulation_1.
+  by rewrite -2!prod_fst_snd_eq.
+- simpl in *.
+  find_rewrite.
+  by rewrite map_app.
+- set e0 := {| evt_tr_r_a := _ ; evt_tr_r_l := _ ; evt_tr_r_trace := _ |}.
+  have ->: e0 = tot_map_onet_event_state_trace e' by [].
+  pose s' := Cons e' s0.
+  rewrite (tot_map_onet_event_state_trace_Map_unfold s').
+  exact: c.
+Qed.
+
+Lemma tot_map_onet_label_event_state_trace_inf_often_occurred :
+  forall l s,
+    inf_often (now (occurred l)) s ->
+    inf_often (now (occurred (tot_map_label l))) (Map tot_map_onet_event_state_trace s).
+Proof.
+move => l.
+apply: always_Map.
+apply: eventually_Map.
+case => e s.
+rewrite /= /occurred /=.
+move => H_eq.
+by rewrite H_eq.
+Qed.
+
+Lemma tot_map_onet_label_event_state_trace_inf_often_occurred_conv :
+  forall l s,
+    inf_often (now (occurred (tot_map_label l))) (Map tot_map_onet_event_state_trace s) ->
+    inf_often (now (occurred l)) s.
+Proof.
+move => l.
+apply: always_Map_conv.
+apply: eventually_Map_conv => //.
+- rewrite /extensional /=.
+  case => e s1.
+  case => e' s2.
+  move => H_eq.
+  by inversion H_eq; subst_max.
+- rewrite /extensional /=.
+  case => e s1.
+  case => e' s2.
+  move => H_eq.
+  by inversion H_eq; subst_max.
+- case => e s.
+  rewrite /= /occurred /=.
+  move => H_eq.
+  exact: tot_map_label_injective.
+Qed.
+
+Context {overlay_fst : NameOverlayParams (@unlabeled_multi_params _ labeled_multi_fst)}.
+Context {overlay_snd : NameOverlayParams (@unlabeled_multi_params _ labeled_multi_snd)}.
+Context {overlay_map_congr : NameOverlayParamsTotalMapCongruency overlay_fst overlay_snd name_map}.
+
+Context {fail_msg_fst : FailMsgParams (@unlabeled_multi_params _ labeled_multi_fst)}.
+Context {fail_msg_snd : FailMsgParams (@unlabeled_multi_params _ labeled_multi_snd)}.
+Context {fail_msg_map_congr : FailMsgParamsTotalMapCongruency fail_msg_fst fail_msg_snd msg_map}.
+  
+Lemma tot_map_onet_hd_step_o_f_star_ex_always : 
+  forall s, event_step_star_ex step_o_f step_o_f_init (hd s) ->
+       lb_step_state_execution lb_step_o_f s ->
+       always (now (event_step_star_ex step_o_f step_o_f_init)) (Map tot_map_onet_event_state s).
+Proof.
+case => e s H_star H_exec.
+apply: step_o_f_star_ex_lb_step_state_execution.
+  rewrite /= /tot_map_onet_event_state /= /event_step_star_ex /=.
+  rewrite /= /tot_map_onet_event_state /= /event_step_star_ex /= in H_star.
+  break_exists.
+  exists (map (@tot_map_trace_occ _ _ _ _ _ name_map) x).
+  apply: step_o_f_tot_mapped_simulation_star_1 => //.
+  by rewrite -prod_fst_snd_eq.  
+exact: lb_step_state_execution_lb_step_o_f_tot_map_onet_infseq.
+Qed.
+
+Lemma tot_map_onet_hd_step_o_f_star_always : 
+  forall s, event_step_star step_o_f step_o_f_init (hd s) ->
+       lb_step_state_trace_execution lb_step_o_f s ->
+       always (now (event_step_star step_o_f step_o_f_init)) (Map tot_map_onet_event_state_trace s).
+Proof.
+case => e s H_star H_exec.
+apply: step_o_f_star_lb_step_state_trace_execution.
+  rewrite /=.
+  rewrite /tot_map_onet_event_state_trace /= /event_step_star /=.
+  apply: step_o_f_tot_mapped_simulation_star_1.
+  by rewrite -prod_fst_snd_eq.
+exact: lb_step_state_trace_execution_lb_step_o_f_tot_map_onet_infseq.
+Qed.
+
+Definition tot_map_odnet_event_state e :=
+{| evt_r_a := (map tot_map_name (fst e.(evt_r_a)), tot_map_odnet (snd e.(evt_r_a))) ;
+   evt_r_l := tot_map_label e.(evt_r_l) |}.
+
+Lemma tot_map_odnet_event_state_Map_unfold : forall s,
+ Cons (tot_map_odnet_event_state (hd s)) (Map tot_map_odnet_event_state (tl s)) = Map tot_map_odnet_event_state s.
+Proof.
+by move => s; rewrite -Map_Cons /= -{3}(recons s).
+Qed.
+
+Lemma lb_step_state_execution_lb_step_o_d_f_tot_map_odnet_infseq : forall s,
+  lb_step_state_execution lb_step_o_d_f s ->
+  lb_step_state_execution lb_step_o_d_f (Map tot_map_odnet_event_state s).
+Proof.
+cofix c.
+move => s H_exec.
+rewrite -tot_map_odnet_event_state_Map_unfold {1}/tot_map_odnet_event_state /=.
+inversion H_exec; subst => /=.
+rewrite -tot_map_odnet_event_state_Map_unfold /= /tot_map_odnet_event_state /=.
+apply: (@Cons_lb_step_exec _ _ _ _ _ _ _ _ (map tot_map_trace_occ tr)) => /=.
+- apply: lb_step_o_d_f_tot_mapped_simulation_1.
+  by rewrite -2!prod_fst_snd_eq.
+- set e0 := {| evt_r_a := _ ; evt_r_l := _  |}.
+  have ->: e0 = tot_map_odnet_event_state e' by [].
+  pose s' := Cons e' s0.
+  rewrite (tot_map_odnet_event_state_Map_unfold s').
+  exact: c.
+Qed.
+
+Lemma tot_map_odnet_label_event_state_inf_often_occurred :
+  forall l s,
+    inf_often (now (occurred l)) s ->
+    inf_often (now (occurred (tot_map_label l))) (Map tot_map_odnet_event_state s).
+Proof.
+move => l.
+apply: always_Map.
+apply: eventually_Map.
+case => e s.
+rewrite /= /occurred /evt_l /=.
+move => H_eq.
+by rewrite H_eq.
+Qed.
+
+Lemma tot_map_odnet_label_event_state_inf_often_occurred_conv :
+  forall l s,
+    inf_often (now (occurred (tot_map_label l))) (Map tot_map_odnet_event_state s) ->
+    inf_often (now (occurred l)) s.
+Proof.
+move => l.
+apply: always_Map_conv.
+apply: eventually_Map_conv => //.
+- rewrite /extensional /=.
+  case => e s1.
+  case => e' s2.
+  move => H_eq.
+  by inversion H_eq; subst_max.
+- rewrite /extensional /=.
+  case => e s1.
+  case => e' s2.
+  move => H_eq.
+  by inversion H_eq; subst_max.
+- case => e s.
+  rewrite /= /occurred /=.
+  move => H_eq.
+  exact: tot_map_label_injective.
+Qed.
+
+Definition tot_map_odnet_event_state_trace e :=
+{| evt_tr_r_a := (map tot_map_name (fst e.(evt_tr_r_a)), tot_map_odnet (snd e.(evt_tr_r_a))) ;
+   evt_tr_r_l := tot_map_label e.(evt_tr_r_l) ;
+   evt_tr_r_trace := map tot_map_trace_occ e.(evt_tr_r_trace) |}.
+
+Lemma tot_map_odnet_event_state_trace_Map_unfold : forall s,
+ Cons (tot_map_odnet_event_state_trace (hd s)) (Map tot_map_odnet_event_state_trace (tl s)) = Map tot_map_odnet_event_state_trace s.
+Proof.
+by move => s; rewrite -Map_Cons /= -{3}(recons s).
+Qed.
+
+Lemma lb_step_state_trace_execution_lb_step_o_d_f_tot_map_odnet_infseq : forall s,
+  lb_step_state_trace_execution lb_step_o_d_f s ->
+  lb_step_state_trace_execution lb_step_o_d_f (Map tot_map_odnet_event_state_trace s).
+Proof.
+cofix c.
+move => s H_exec.
+rewrite -tot_map_odnet_event_state_trace_Map_unfold {1}/tot_map_odnet_event_state_trace /=.
+inversion H_exec; subst => /=.
+rewrite -tot_map_odnet_event_state_trace_Map_unfold /= /tot_map_odnet_event_state_trace /=.
+apply: (@Cons_lb_step_trace_exec _ _ _ _ _ _ _ _ (map tot_map_trace_occ tr)) => /=.
+- apply: lb_step_o_d_f_tot_mapped_simulation_1.
+  by rewrite -2!prod_fst_snd_eq.
+- simpl in *.
+  find_rewrite.
+  by rewrite map_app.
+- set e0 := {| evt_tr_r_a := _ ; evt_tr_r_l := _ ; evt_tr_r_trace := _ |}.
+  have ->: e0 = tot_map_odnet_event_state_trace e' by [].
+  pose s' := Cons e' s0.
+  rewrite (tot_map_odnet_event_state_trace_Map_unfold s').
+  exact: c.
+Qed.
+
+Lemma tot_map_odnet_label_event_state_trace_inf_often_occurred :
+  forall l s,
+    inf_often (now (occurred l)) s ->
+    inf_often (now (occurred (tot_map_label l))) (Map tot_map_odnet_event_state_trace s).
+Proof.
+move => l.
+apply: always_Map.
+apply: eventually_Map.
+case => e s.
+rewrite /= /occurred /=.
+move => H_eq.
+by rewrite H_eq.
+Qed.
+
+Lemma tot_map_odnet_label_event_state_trace_inf_often_occurred_conv :
+  forall l s,
+    inf_often (now (occurred (tot_map_label l))) (Map tot_map_odnet_event_state_trace s) ->
+    inf_often (now (occurred l)) s.
+Proof.
+move => l.
+apply: always_Map_conv.
+apply: eventually_Map_conv => //.
+- rewrite /extensional /=.
+  case => e s1.
+  case => e' s2.
+  move => H_eq.
+  by inversion H_eq; subst_max.
+- rewrite /extensional /=.
+  case => e s1.
+  case => e' s2.
+  move => H_eq.
+  by inversion H_eq; subst_max.
+- case => e s.
+  rewrite /= /occurred /=.
+  move => H_eq.
+  exact: tot_map_label_injective.
+Qed.
+
+Context {new_msg_fst : NewMsgParams (@unlabeled_multi_params _ labeled_multi_fst)}.
+Context {new_msg_snd : NewMsgParams (@unlabeled_multi_params _ labeled_multi_snd)}.
+Context {new_msg_map_congr : NewMsgParamsTotalMapCongruency new_msg_fst new_msg_snd msg_map}.
+
+Lemma tot_map_odnet_hd_step_o_d_f_star_ex_always : 
+  forall s, event_step_star_ex step_o_d_f step_o_d_f_init (hd s) ->
+       lb_step_state_execution lb_step_o_d_f s ->
+       always (now (event_step_star_ex step_o_d_f step_o_d_f_init)) (Map tot_map_odnet_event_state s).
+Proof.
+case => e s H_star H_exec.
+apply: step_o_d_f_star_ex_lb_step_state_execution.
+  rewrite /= /tot_map_odnet_event_state /= /event_step_star_ex /=.
+  rewrite /= /tot_map_odnet_event_state /= /event_step_star_ex /= in H_star.
+  break_exists.
+  exists (map (@tot_map_trace_occ _ _ _ _ _ name_map) x).
+  apply: step_o_d_f_tot_mapped_simulation_star_1 => //.
+  by rewrite -prod_fst_snd_eq.  
+exact: lb_step_state_execution_lb_step_o_d_f_tot_map_odnet_infseq.
+Qed.
+
+Lemma tot_map_odnet_hd_step_o_d_f_star_always : 
+  forall s, event_step_star step_o_d_f step_o_d_f_init (hd s) ->
+       lb_step_state_trace_execution lb_step_o_d_f s ->
+       always (now (event_step_star step_o_d_f step_o_d_f_init)) (Map tot_map_odnet_event_state_trace s).
+Proof.
+case => e s H_star H_exec.
+apply: step_o_d_f_star_lb_step_state_trace_execution.
+  rewrite /=.
+  rewrite /tot_map_odnet_event_state_trace /= /event_step_star /=.
+  apply: step_o_d_f_tot_mapped_simulation_star_1.
+  by rewrite -prod_fst_snd_eq.
+exact: lb_step_state_trace_execution_lb_step_o_d_f_tot_map_odnet_infseq.
 Qed.
 
 End TotalMapLivenessSimulations.
